fix

Logic/IntProp/Heyting/Semantics.lean
@@ -12,8 +12,8 @@ def hVal {ℍ : Type*} [HeytingAlgebra ℍ] (v : α → ℍ) : Formula α → �
   | ⊥      => ⊥
   | p ⋏ q  => p.hVal v ⊓ q.hVal v
   | p ⋎ q  => p.hVal v ⊔ q.hVal v
-  | p ⟶ q  => p.hVal v ⇨ q.hVal v
-  | ~p     => (p.hVal v)ᶜ
+  | p ➝ q  => p.hVal v ⇨ q.hVal v
+  | ∼p     => (p.hVal v)ᶜ
 
 variable {ℍ : Type*} [HeytingAlgebra ℍ] (v : α → ℍ)
 
@@ -27,9 +27,9 @@ variable {ℍ : Type*} [HeytingAlgebra ℍ] (v : α → ℍ)
 
 @[simp] lemma hVal_or (p q : Formula α) : (p ⋎ q).hVal v = p.hVal v ⊔ q.hVal v := rfl
 
-@[simp] lemma hVal_imp (p q : Formula α) : (p ⟶ q).hVal v = p.hVal v ⇨ q.hVal v := rfl
+@[simp] lemma hVal_imp (p q : Formula α) : (p ➝ q).hVal v = p.hVal v ⇨ q.hVal v := rfl
 
-@[simp] lemma hVal_neg (p : Formula α) : (~p).hVal v = (p.hVal v)ᶜ := rfl
+@[simp] lemma hVal_neg (p : Formula α) : (∼p).hVal v = (p.hVal v)ᶜ := rfl
 
 end Formula
 
@@ -37,20 +37,39 @@ structure HeytingSemantics (α : Type*) where
   Algebra : Type*
   valAtom : α → Algebra
   [heyting : HeytingAlgebra Algebra]
+  [nontrivial : Nontrivial Algebra]
 
 namespace HeytingSemantics
 
+variable (ℍ : HeytingSemantics α)
+
 instance : CoeSort (HeytingSemantics α) (Type _) := ⟨Algebra⟩
 
-instance (ℍ : HeytingSemantics α) : HeytingAlgebra ℍ := ℍ.heyting
+instance : HeytingAlgebra ℍ := ℍ.heyting
 
-def Val (ℍ : HeytingSemantics α) (p : Formula α) : Prop := p.hVal ℍ.valAtom = ⊤
+instance : Nontrivial ℍ := ℍ.nontrivial
 
-instance : Semantics (Formula α) (HeytingSemantics α) := ⟨Val⟩
+def val (ℍ : HeytingSemantics α) (p : Formula α) : ℍ := p.hVal ℍ.valAtom
+
+scoped [LO.IntProp] infix:45 " ⊧ₕ " => LO.IntProp.HeytingSemantics.val
+
+@[simp] lemma val_verum : (ℍ ⊧ₕ ⊤) = ⊤ := rfl
+
+@[simp] lemma val_falsum : (ℍ ⊧ₕ ⊥) = ⊥ := rfl
+
+@[simp] lemma val_and (p q : Formula α) : (ℍ ⊧ₕ p ⋏ q) = (ℍ ⊧ₕ p) ⊓ (ℍ ⊧ₕ q) := rfl
+
+@[simp] lemma val_or (p q : Formula α) : (ℍ ⊧ₕ p ⋎ q) = (ℍ ⊧ₕ p) ⊔ (ℍ ⊧ₕ q) := rfl
+
+@[simp] lemma val_imply (p q : Formula α) : (ℍ ⊧ₕ p ➝ q) = (ℍ ⊧ₕ p) ⇨ (ℍ ⊧ₕ q) := rfl
+
+instance : Semantics (Formula α) (HeytingSemantics α) := ⟨fun ℍ p ↦ (ℍ ⊧ₕ p) = ⊤⟩
 
 lemma val_def (ℍ : HeytingSemantics α) (p : Formula α) : ℍ ⊧ p ↔ p.hVal ℍ.valAtom = ⊤ := by rfl
 
 instance : Semantics.Top (HeytingSemantics α) := ⟨fun ℍ ↦ by simp [val_def]⟩
+
+instance : Semantics.Bot (HeytingSemantics α) := ⟨fun ℍ ↦ by simp [val_def]⟩
 
 instance : Semantics.And (HeytingSemantics α) := ⟨fun {ℍ p q} ↦ by simp [val_def]⟩
 
